\question

\begin{arabicparts}

    \questionpart
    \renewcommand{\labelenumii}{(\alph{enumii})}
    \begin{enumerate}
        \setcounter{enumii}{1}
        \item $\eventually\finally (\phi \lor \psi) \equiv \eventually\finally
        \phi \lor \eventually\finally \psi$ --- Equivalent, proved earlier.

        \item $\always\globally (\phi \lor \psi) \equiv \always\globally \phi
            \lor \eventually\finally \psi$ --- Equivalent.
        
        \setcounter{enumii}{6}
        \item $\top \equiv \always\globally\phi \Rightarrow \eventually\globally\phi$ --- Equivalent.
        
        \item $\top \equiv \eventually\globally\phi \Rightarrow
            \always\globally\phi$ --- Not equivalent. Consider the model in
            \autoref{fig:q4ts} and take the initial state to be $s_1$, with
            $\phi = r$. The self-loop causes $\eventually\globally \phi$ to
            hold, but on no other path does $\globally\phi$ hold, so the
            implication breaks.
    \end{enumerate}

    \questionpart 
    \begin{enumerate}
        \item $\always\globally (\phi \land \psi) \equiv \always\globally \phi ? \always\globally \psi$ --- $? \rightarrow \land$
        \item $\eventually\finally\lnot\phi \equiv \lnot ?? \phi$ --- $?? \rightarrow \always\globally$
    \end{enumerate}

\end{arabicparts}